examples/low-level/sieve.fst
@@ -1,6 +1,6 @@
 (*--build-config
     other-files:ext.fst set.fsi set.fst heap.fst st.fst all.fst list.fst  stack.fst listset.fst
-    ghost.fst located.fst lref.fst stackAndHeap.fst sst.fst sstCombinators.fst seq.fsi seq.fst array.fsi array.fst arrayalgos.fst sieveFun.fst
+    ghost.fst located.fst lref.fst stackAndHeap.fst sst.fst rstWhile.fst seq.fsi seq.fst array.fsi array.fst arrayalgos.fst sieveFun.fst
   --*)
 module Sieve
 open RSTCombinators
